Towards proving properties of jscert states.

LambdaS5/coq/JsBagAdapter.v
@@ -2,16 +2,32 @@ Require Import Utils.
 Require Import LibBagExt.
 Require Import JsSyntax.
 Require Import JsPreliminary.
+Import LibStream.
+
+Module Import JsCertExt.
+
+Definition state_fresh_object_loc jst := object_loc_normal (LibStream.stream_head (state_fresh_locations jst)).
+
+Definition state_fresh_env_record_loc jst : env_loc := LibStream.stream_head (state_fresh_locations jst).
+
+Definition state_next_fresh jst :=
+    match jst with
+    | state_intro oh eh (LibStream.stream_intro _ fl) el => state_intro oh eh fl el
+    end.
+
+Definition env_record_indom S L :=
+    Heap.indom (state_env_record_heap S) L.
+
+Definition state_fresh_ok jst := LibStream.always 
+    (fun fl => ~object_indom jst (object_loc_normal (LibStream.stream_head fl)) /\ 
+        ~env_record_indom jst (LibStream.stream_head fl)) 
+    (state_fresh_locations jst).
+
+End JsCertExt.
 
 Section Instances.
 
 Variables (A B : Type).
-
-Global Instance binds_object_inst : BagBinds object_loc object state :=
-    { binds := object_binds }.
-
-Global Instance binds_env_record_inst : BagBinds env_loc env_record state :=
-    { binds := env_record_binds }.
 
 Global Instance binds_heap_inst : BagBinds A B (Heap.heap A B) :=
     { binds := @Heap.binds _ _ }.
@@ -22,10 +38,91 @@ Global Instance index_heap_inst : BagIndex (Heap.heap A B) A :=
 Global Instance dom_heap_inst : BagDom (Heap.heap A B) (set A) :=
     { dom := @Heap.dom _ _ }.
 
+Global Instance update_heap_inst : BagUpdate A B (Heap.heap A B) :=
+    { update := @Heap.write _ _ }.
+
 Global Instance dom_index_eq_inst : Dom_index_eq.
 Admitted. (* TODO *)
 
 Global Instance index_binds_eq_inst : Index_binds_eq.
 Admitted. (* TODO *)
 
+Global Instance binds_update_eq_inst : Binds_update_eq.
+Admitted. (* TODO *)
+
 End Instances.
+
+Section StateInstances.
+
+Global Instance binds_object_state_inst : BagBinds object_loc object state :=
+    { binds := object_binds }.
+
+Global Instance binds_env_record_state_inst : BagBinds env_loc env_record state :=
+    { binds := env_record_binds }.
+
+Global Instance index_object_state_inst : BagIndex state object_loc :=
+    { index := object_indom }.
+
+Global Instance index_env_record_state_inst : BagIndex state env_loc :=
+    { index := env_record_indom }.
+
+Global Instance update_object_state_inst : BagUpdate object_loc object state :=
+    { update := object_write }.
+
+Global Instance update_env_record_state_inst : BagUpdate env_loc env_record state :=
+    { update := env_record_write }.
+
+Global Instance fresh_object_state_inst : BagFresh object_loc state :=
+    { fresh := state_fresh_object_loc }.
+
+Global Instance fresh_env_record_state_inst : BagFresh env_loc state :=
+    { fresh := state_fresh_env_record_loc }.
+
+Global Instance index_binds_eq_object_state_inst : Index_binds_eq (T := state) (A := object_loc).
+Proof. 
+    constructor. introv. 
+    applys (index_binds_eq (T := Heap.heap object_loc object)).
+Qed.
+
+Global Instance index_binds_eq_env_record_state_inst : Index_binds_eq (T := state) (A := env_loc).
+Proof. 
+    constructor. introv. 
+    applys (index_binds_eq (T := Heap.heap env_loc env_record)).
+Qed.
+
+Global Instance binds_update_eq_object_state_inst : Binds_update_eq (T := state) (A := object_loc).
+Proof.
+    constructor. introv.
+    destruct M.
+    applys (binds_update_eq (T := Heap.heap object_loc object)).
+Qed.
+
+Global Instance binds_update_eq_env_record_state_inst : Binds_update_eq (T := state) (A := env_loc).
+Proof.
+    constructor. introv.
+    destruct M.
+    applys (binds_update_eq (T := Heap.heap env_loc env_record)).
+Qed.
+
+End StateInstances.
+
+Lemma js_state_fresh_ok_next_fresh_preserved : forall jst, 
+    state_fresh_ok jst -> state_fresh_ok (state_next_fresh jst).
+Proof.
+    introv Hfok.
+    unfolds state_fresh_ok.
+    destruct jst.
+    simpls.
+    inverts Hfok.
+    eauto.
+Qed.
+
+Lemma js_object_alloc_lemma : forall jst jobj,
+    (object_loc_normal (fresh jst), state_next_fresh (jst \(fresh jst := jobj))) =
+    JsPreliminary.object_alloc jst jobj.
+Proof.
+    introv.
+    destruct jst. destruct state_fresh_locations.
+    reflexivity.
+Qed.
+
